examples/dll_singleton.v
@@ -9,19 +9,19 @@ Require Import core.
 
 Inductive dll (x : ptr) (z : ptr) (s : seq nat) (h : heap) : Prop :=
 | dll1 of x == null of
-  perm_eq (s) (nil) /\ h = empty
+  @perm_eq nat_eqType (s) (nil) /\ h = empty
 | dll2 of ~~ (x == null) of
   exists (v : nat) (s1 : seq nat) (w : ptr),
   exists h_dll_wxs1_549,
-  perm_eq (s) ([:: v] ++ s1) /\ h = x :-> v \+ x .+ 1 :-> w \+ x .+ 2 :-> z \+ h_dll_wxs1_549 /\ dll w x s1 h_dll_wxs1_549.
+  @perm_eq nat_eqType (s) ([:: v] ++ s1) /\ h = x :-> v \+ x .+ 1 :-> w \+ x .+ 2 :-> z \+ h_dll_wxs1_549 /\ dll w x s1 h_dll_wxs1_549.
 
 Inductive sll (x : ptr) (s : seq nat) (h : heap) : Prop :=
 | sll1 of x == null of
-  perm_eq (s) (nil) /\ h = empty
+  @perm_eq nat_eqType (s) (nil) /\ h = empty
 | sll2 of ~~ (x == null) of
   exists (v : nat) (s1 : seq nat) (nxt : ptr),
   exists h_sll_nxts1_550,
-  perm_eq (s) ([:: v] ++ s1) /\ h = x :-> v \+ x .+ 1 :-> nxt \+ h_sll_nxts1_550 /\ sll nxt s1 h_sll_nxts1_550.
+  @perm_eq nat_eqType (s) ([:: v] ++ s1) /\ h = x :-> v \+ x .+ 1 :-> nxt \+ h_sll_nxts1_550 /\ sll nxt s1 h_sll_nxts1_550.
 
 Definition dll_singleton_type :=
   forall (vprogs : nat * ptr),
@@ -36,7 +36,7 @@ Definition dll_singleton_type :=
       let: (a) := vghosts in
       exists elems y,
       exists h_dll_yelems_551,
-      perm_eq (elems) ([:: x]) /\ h = r :-> y \+ h_dll_yelems_551 /\ dll y null elems h_dll_yelems_551
+      @perm_eq nat_eqType (elems) ([:: x]) /\ h = r :-> y \+ h_dll_yelems_551 /\ dll y null elems h_dll_yelems_551
     ]).
 Program Definition dll_singleton : dll_singleton_type :=
   Fix (fun (dll_singleton : dll_singleton_type) vprogs =>
@@ -51,6 +51,10 @@ Program Definition dll_singleton : dll_singleton_type :=
     )).
 Obligation Tactic := intro; move=>[x r]; ssl_program_simpl.
 Next Obligation.
+Hypothesis dll_perm_eq_trans35: forall x z h s_1 s_2, perm_eq s_1 s_2 -> dll x z s_1 h -> dll x z s_2 h.
+Hint Resolve dll_perm_eq_trans35: ssl_pred.
+Hypothesis sll_perm_eq_trans36: forall x h s_1 s_2, perm_eq s_1 s_2 -> sll x s_1 h -> sll x s_2 h.
+Hint Resolve sll_perm_eq_trans36: ssl_pred.
 ssl_ghostelim_pre.
 move=>a2.
 move=>[sigma_self].
@@ -63,6 +67,8 @@ ssl_write (y2 .+ 1).
 ssl_write_post (y2 .+ 1).
 ssl_write (y2 .+ 2).
 ssl_write_post (y2 .+ 2).
+Hypothesis pure37 : forall x, @perm_eq nat_eqType ([:: x]) ([:: x]).
+Hint Resolve pure37: ssl_pure.
 ssl_write y2.
 ssl_write_post y2.
 ssl_emp;
@@ -75,5 +81,4 @@ exists (empty);
 sslauto.
 unfold_constructor 1;
 sslauto.
-
 Qed.
