examples/sll_append.v
@@ -9,31 +9,27 @@ Require Import core.
 
 Inductive sll (x : ptr) (s : seq nat) (h : heap) : Prop :=
 | sll1 of x == null of
-  perm_eq (s) (nil) /\ h = empty
+  @perm_eq nat_eqType (s) (nil) /\ h = empty
 | sll2 of ~~ (x == null) of
   exists (v : nat) (s1 : seq nat) (nxt : ptr),
   exists h_sll_nxts1_537,
-  perm_eq (s) ([:: v] ++ s1) /\ h = x :-> v \+ x .+ 1 :-> nxt \+ h_sll_nxts1_537 /\ sll nxt s1 h_sll_nxts1_537.
-
-(* TODO: autogenerate *)
-Hypothesis sll_perm_eq: forall s x h s1, perm_eq s s1 -> sll x s h -> sll x s1 h.
-Hint Resolve sll_perm_eq : ssl_pred.
+  @perm_eq nat_eqType (s) ([:: v] ++ s1) /\ h = x :-> v \+ x .+ 1 :-> nxt \+ h_sll_nxts1_537 /\ sll nxt s1 h_sll_nxts1_537.
 
 Definition sll_append_type :=
   forall (vprogs : ptr * ptr),
-  {(vghosts : seq nat * seq nat * ptr)},
+  {(vghosts : seq nat * ptr * seq nat)},
   STsep (
     fun h =>
       let: (x1, r) := vprogs in
-      let: (s1, s2, x2) := vghosts in
+      let: (s1, x2, s2) := vghosts in
       exists h_sll_x1s1_538 h_sll_x2s2_539,
       h = r :-> x2 \+ h_sll_x1s1_538 \+ h_sll_x2s2_539 /\ sll x1 s1 h_sll_x1s1_538 /\ sll x2 s2 h_sll_x2s2_539,
     [vfun (_: unit) h =>
       let: (x1, r) := vprogs in
-      let: (s1, s2, x2) := vghosts in
+      let: (s1, x2, s2) := vghosts in
       exists s y,
       exists h_sll_ys_540,
-      perm_eq (s) (s1 ++ s2) /\ h = r :-> y \+ h_sll_ys_540 /\ sll y s h_sll_ys_540
+      @perm_eq nat_eqType (s) (s1 ++ s2) /\ h = r :-> y \+ h_sll_ys_540 /\ sll y s h_sll_ys_540
     ]).
 Program Definition sll_append : sll_append_type :=
   Fix (fun (sll_append : sll_append_type) vprogs =>
@@ -52,8 +48,10 @@ Program Definition sll_append : sll_append_type :=
     )).
 Obligation Tactic := intro; move=>[x1 r]; ssl_program_simpl.
 Next Obligation.
+Hypothesis sll_perm_eq_trans25: forall x h s_1 s_2, perm_eq s_1 s_2 -> sll x s_1 h -> sll x s_2 h.
+Hint Resolve sll_perm_eq_trans25: ssl_pred.
 ssl_ghostelim_pre.
-move=>[[s1 s2] x22].
+move=>[[s1 x22] s2].
 ex_elim h_sll_x1s1_538 h_sll_x22s2_539.
 move=>[sigma_self].
 subst.
@@ -61,7 +59,7 @@ move=>[H_sll_x1s1_538 H_sll_x22s2_539].
 ssl_ghostelim_post.
 ssl_open.
 ssl_open_post H_sll_x1s1_538.
-move=>[phi_sll_x1s1_538].
+move=>[phi_sll_x1s1_5380].
 move=>[sigma_sll_x1s1_538].
 subst.
 ssl_emp;
@@ -71,21 +69,21 @@ sslauto.
 ssl_open_post H_sll_x1s1_538.
 ex_elim vx12 s1x1 nxtx12.
 ex_elim h_sll_nxtx12s1x1_537x1.
-move=>[phi_sll_x1s1_538].
+move=>[phi_sll_x1s1_5380].
 move=>[sigma_sll_x1s1_538].
 subst.
 move=>H_sll_nxtx12s1x1_537x1.
 ssl_read (x1 .+ 1).
 ssl_call_pre (r :-> x22 \+ h_sll_nxtx12s1x1_537x1 \+ h_sll_x22s2_539).
-ssl_call (s1x1, s2, x22).
+ssl_call (s1x1, x22, s2).
 exists (h_sll_nxtx12s1x1_537x1);
 exists (h_sll_x22s2_539);
 sslauto.
-move=>h_call11.
+move=>h_call1.
 ex_elim s3 y12.
-ex_elim h_sll_y12s3_5401.
-move=>[phi_call11].
-move=>[sigma_call11].
+ex_elim h_sll_y12s1x1s2_5401.
+move=>[phi_call10].
+move=>[sigma_call1].
 subst.
 move=>H_sll_y12s3_5401.
 store_valid.
@@ -94,13 +92,14 @@ ssl_write (x1 .+ 1).
 ssl_write_post (x1 .+ 1).
 ssl_write r.
 ssl_write_post r.
+Hypothesis pure26 : forall vx12 s1x1 s2, @perm_eq nat_eqType ([:: vx12] ++ s1x1 ++ s2) ([:: vx12] ++ s1x1 ++ s2).
+Hint Resolve pure26: ssl_pure.
 ssl_emp;
 exists ([:: vx12] ++ s1x1 ++ s2), (x1);
-(* TODO: predicate assertion naming issue *)  
-exists (x1 :-> vx12 \+ x1 .+ 1 :-> y12 \+ (*h_sll_y12s1x1s2_5401*) h_sll_y12s3_5401);
+exists (x1 :-> vx12 \+ x1 .+ 1 :-> y12 \+ h_sll_y12s1x1s2_5401);
 sslauto.
 unfold_constructor 2;
 exists (vx12), (s1x1 ++ s2), (y12);
-exists ((*h_sll_y12s1x1s2_5401*) h_sll_y12s3_5401);
+exists (h_sll_y12s1x1s2_5401);
 sslauto.
 Qed.
