examples/sll_dupleton.v
@@ -9,11 +9,11 @@ Require Import core.
 
 Inductive sll (x : ptr) (s : seq nat) (h : heap) : Prop :=
 | sll1 of x == null of
-  perm_eq (s) (nil) /\ h = empty
+  @perm_eq nat_eqType (s) (nil) /\ h = empty
 | sll2 of ~~ (x == null) of
   exists (v : nat) (s1 : seq nat) (nxt : ptr),
   exists h_sll_nxts1_532,
-  perm_eq (s) ([:: v] ++ s1) /\ h = x :-> v \+ x .+ 1 :-> nxt \+ h_sll_nxts1_532 /\ sll nxt s1 h_sll_nxts1_532.
+  @perm_eq nat_eqType (s) ([:: v] ++ s1) /\ h = x :-> v \+ x .+ 1 :-> nxt \+ h_sll_nxts1_532 /\ sll nxt s1 h_sll_nxts1_532.
 
 Definition sll_dupleton_type :=
   forall (vprogs : nat * nat * ptr),
@@ -28,7 +28,7 @@ Definition sll_dupleton_type :=
       let: (a) := vghosts in
       exists elems z,
       exists h_sll_zelems_533,
-      perm_eq (elems) ([:: x; y]) /\ h = r :-> z \+ h_sll_zelems_533 /\ sll z elems h_sll_zelems_533
+      @perm_eq nat_eqType (elems) ([:: x; y]) /\ h = r :-> z \+ h_sll_zelems_533 /\ sll z elems h_sll_zelems_533
     ]).
 Program Definition sll_dupleton : sll_dupleton_type :=
   Fix (fun (sll_dupleton : sll_dupleton_type) vprogs =>
@@ -45,6 +45,8 @@ Program Definition sll_dupleton : sll_dupleton_type :=
     )).
 Obligation Tactic := intro; move=>[[x y] r]; ssl_program_simpl.
 Next Obligation.
+Hypothesis sll_perm_eq_trans17: forall x h s_1 s_2, perm_eq s_1 s_2 -> sll x s_1 h -> sll x s_2 h.
+Hint Resolve sll_perm_eq_trans17: ssl_pred.
 ssl_ghostelim_pre.
 move=>a2.
 move=>[sigma_self].
@@ -58,6 +60,8 @@ ssl_write (z2 .+ 1).
 ssl_write_post (z2 .+ 1).
 ssl_write (nxtz2 .+ 1).
 ssl_write_post (nxtz2 .+ 1).
+Hypothesis pure18 : forall x y, @perm_eq nat_eqType ([:: x; y]) ([:: x] ++ [:: y]).
+Hint Resolve pure18: ssl_pure.
 ssl_write z2.
 ssl_write_post z2.
 ssl_write nxtz2.
@@ -76,5 +80,4 @@ exists (empty);
 sslauto.
 unfold_constructor 1;
 sslauto.
-
 Qed.
