examples/sll_free.v
@@ -9,11 +9,11 @@ Require Import core.
 
 Inductive sll (x : ptr) (s : seq nat) (h : heap) : Prop :=
 | sll1 of x == null of
-  perm_eq (s) (nil) /\ h = empty
+  @perm_eq nat_eqType (s) (nil) /\ h = empty
 | sll2 of ~~ (x == null) of
   exists (v : nat) (s1 : seq nat) (nxt : ptr),
   exists h_sll_nxts1_535,
-  perm_eq (s) ([:: v] ++ s1) /\ h = x :-> v \+ x .+ 1 :-> nxt \+ h_sll_nxts1_535 /\ sll nxt s1 h_sll_nxts1_535.
+  @perm_eq nat_eqType (s) ([:: v] ++ s1) /\ h = x :-> v \+ x .+ 1 :-> nxt \+ h_sll_nxts1_535 /\ sll nxt s1 h_sll_nxts1_535.
 
 Definition sll_free_type :=
   forall (vprogs : ptr),
@@ -45,6 +45,8 @@ Program Definition sll_free : sll_free_type :=
     )).
 Obligation Tactic := intro; move=>x; ssl_program_simpl.
 Next Obligation.
+Hypothesis sll_perm_eq_trans24: forall x h s_1 s_2, perm_eq s_1 s_2 -> sll x s_1 h -> sll x s_2 h.
+Hint Resolve sll_perm_eq_trans24: ssl_pred.
 ssl_ghostelim_pre.
 move=>s.
 ex_elim h_sll_xs_536.
@@ -54,7 +56,7 @@ move=>H_sll_xs_536.
 ssl_ghostelim_post.
 ssl_open.
 ssl_open_post H_sll_xs_536.
-move=>[phi_sll_xs_536].
+move=>[phi_sll_xs_5360].
 move=>[sigma_sll_xs_536].
 subst.
 ssl_emp;
@@ -62,7 +64,7 @@ sslauto.
 ssl_open_post H_sll_xs_536.
 ex_elim vx2 s1x nxtx2.
 ex_elim h_sll_nxtx2s1x_535x.
-move=>[phi_sll_xs_536].
+move=>[phi_sll_xs_5360].
 move=>[sigma_sll_xs_536].
 subst.
 move=>H_sll_nxtx2s1x_535x.
@@ -71,13 +73,12 @@ ssl_call_pre (h_sll_nxtx2s1x_535x).
 ssl_call (s1x).
 exists (h_sll_nxtx2s1x_535x);
 sslauto.
-move=>h_call10.
-move=>[sigma_call10].
+move=>h_call1.
+move=>[sigma_call1].
 subst.
 store_valid.
-ssl_dealloc (x).
+ssl_dealloc x.
 ssl_dealloc (x .+ 1).
 ssl_emp;
 sslauto.
-
 Qed.
