examples/sll_init.v
@@ -9,11 +9,11 @@ Require Import core.
 
 Inductive sll (x : ptr) (s : seq nat) (h : heap) : Prop :=
 | sll1 of x == null of
-  perm_eq (s) (nil) /\ h = empty
+  @perm_eq nat_eqType (s) (nil) /\ h = empty
 | sll2 of ~~ (x == null) of
   exists (v : nat) (s1 : seq nat) (nxt : ptr),
   exists h_sll_nxts1_543,
-  perm_eq (s) ([:: v] ++ s1) /\ h = x :-> v \+ x .+ 1 :-> nxt \+ h_sll_nxts1_543 /\ sll nxt s1 h_sll_nxts1_543.
+  @perm_eq nat_eqType (s) ([:: v] ++ s1) /\ h = x :-> v \+ x .+ 1 :-> nxt \+ h_sll_nxts1_543 /\ sll nxt s1 h_sll_nxts1_543.
 
 Definition sll_init_type :=
   forall (vprogs : ptr * nat),
@@ -29,7 +29,7 @@ Definition sll_init_type :=
       let: (s) := vghosts in
       exists s1,
       exists h_sll_xs1_545,
-      {subset s1 <= [:: v]} /\ h = h_sll_xs1_545 /\ sll x s1 h_sll_xs1_545
+      @sub_mem nat_eqType (mem (s1)) (mem ([:: v])) /\ h = h_sll_xs1_545 /\ sll x s1 h_sll_xs1_545
     ]).
 Program Definition sll_init : sll_init_type :=
   Fix (fun (sll_init : sll_init_type) vprogs =>
@@ -46,6 +46,8 @@ Program Definition sll_init : sll_init_type :=
     )).
 Obligation Tactic := intro; move=>[x v]; ssl_program_simpl.
 Next Obligation.
+Hypothesis sll_perm_eq_trans29: forall x h s_1 s_2, perm_eq s_1 s_2 -> sll x s_1 h -> sll x s_2 h.
+Hint Resolve sll_perm_eq_trans29: ssl_pred.
 ssl_ghostelim_pre.
 move=>s.
 ex_elim h_sll_xs_544.
@@ -55,9 +57,11 @@ move=>H_sll_xs_544.
 ssl_ghostelim_post.
 ssl_open.
 ssl_open_post H_sll_xs_544.
-move=>[phi_sll_xs_544].
+move=>[phi_sll_xs_5440].
 move=>[sigma_sll_xs_544].
 subst.
+Hypothesis pure30 : forall v, @sub_mem nat_eqType (mem (nil)) (mem ([:: v])).
+Hint Resolve pure30: ssl_pure.
 ssl_emp;
 exists (nil);
 exists (empty);
@@ -67,7 +71,7 @@ sslauto.
 ssl_open_post H_sll_xs_544.
 ex_elim vx2 s1x nxtx2.
 ex_elim h_sll_nxtx2s1x_543x.
-move=>[phi_sll_xs_544].
+move=>[phi_sll_xs_5440].
 move=>[sigma_sll_xs_544].
 subst.
 move=>H_sll_nxtx2s1x_543x.
@@ -76,14 +80,16 @@ ssl_call_pre (h_sll_nxtx2s1x_543x).
 ssl_call (s1x).
 exists (h_sll_nxtx2s1x_543x);
 sslauto.
-move=>h_call12.
+move=>h_call1.
 ex_elim s11.
 ex_elim h_sll_nxtx2s11_5451.
-move=>[phi_call12].
-move=>[sigma_call12].
+move=>[phi_call10].
+move=>[sigma_call1].
 subst.
 move=>H_sll_nxtx2s11_5451.
 store_valid.
+Hypothesis pure31 : forall v s11, @sub_mem nat_eqType (mem (s11)) (mem ([:: v])) -> @sub_mem nat_eqType (mem ([:: v] ++ s11)) (mem ([:: v])).
+Hint Resolve pure31: ssl_pure.
 ssl_write x.
 ssl_write_post x.
 ssl_emp;
@@ -94,5 +100,4 @@ unfold_constructor 2;
 exists (v), (s11), (nxtx2);
 exists (h_sll_nxtx2s11_5451);
 sslauto.
-
 Qed.
