examples/sll_to_dll.v
@@ -9,19 +9,19 @@ Require Import core.
 
 Inductive dll (x : ptr) (z : ptr) (s : seq nat) (h : heap) : Prop :=
 | dll1 of x == null of
-  perm_eq (s) (nil) /\ h = empty
+  @perm_eq nat_eqType (s) (nil) /\ h = empty
 | dll2 of ~~ (x == null) of
   exists (v : nat) (s1 : seq nat) (w : ptr),
   exists h_dll_wxs1_552,
-  perm_eq (s) ([:: v] ++ s1) /\ h = x :-> v \+ x .+ 1 :-> w \+ x .+ 2 :-> z \+ h_dll_wxs1_552 /\ dll w x s1 h_dll_wxs1_552.
+  @perm_eq nat_eqType (s) ([:: v] ++ s1) /\ h = x :-> v \+ x .+ 1 :-> w \+ x .+ 2 :-> z \+ h_dll_wxs1_552 /\ dll w x s1 h_dll_wxs1_552.
 
 Inductive sll (x : ptr) (s : seq nat) (h : heap) : Prop :=
 | sll1 of x == null of
-  perm_eq (s) (nil) /\ h = empty
+  @perm_eq nat_eqType (s) (nil) /\ h = empty
 | sll2 of ~~ (x == null) of
   exists (v : nat) (s1 : seq nat) (nxt : ptr),
   exists h_sll_nxts1_553,
-  perm_eq (s) ([:: v] ++ s1) /\ h = x :-> v \+ x .+ 1 :-> nxt \+ h_sll_nxts1_553 /\ sll nxt s1 h_sll_nxts1_553.
+  @perm_eq nat_eqType (s) ([:: v] ++ s1) /\ h = x :-> v \+ x .+ 1 :-> nxt \+ h_sll_nxts1_553 /\ sll nxt s1 h_sll_nxts1_553.
 
 Definition sll_to_dll_type :=
   forall (vprogs : ptr),
@@ -76,6 +76,10 @@ Program Definition sll_to_dll : sll_to_dll_type :=
     )).
 Obligation Tactic := intro; move=>f; ssl_program_simpl.
 Next Obligation.
+Hypothesis dll_perm_eq_trans38: forall x z h s_1 s_2, perm_eq s_1 s_2 -> dll x z s_1 h -> dll x z s_2 h.
+Hint Resolve dll_perm_eq_trans38: ssl_pred.
+Hypothesis sll_perm_eq_trans39: forall x h s_1 s_2, perm_eq s_1 s_2 -> sll x s_1 h -> sll x s_2 h.
+Hint Resolve sll_perm_eq_trans39: ssl_pred.
 ssl_ghostelim_pre.
 move=>[x2 s].
 ex_elim h_sll_x2s_554.
@@ -86,9 +90,11 @@ ssl_ghostelim_post.
 ssl_read f.
 ssl_open.
 ssl_open_post H_sll_x2s_554.
-move=>[phi_sll_x2s_554].
+move=>[phi_sll_x2s_5540].
 move=>[sigma_sll_x2s_554].
 subst.
+Hypothesis pure40 : @perm_eq nat_eqType (nil) (nil).
+Hint Resolve pure40: ssl_pure.
 ssl_emp;
 exists (null);
 exists (empty);
@@ -98,7 +104,7 @@ sslauto.
 ssl_open_post H_sll_x2s_554.
 ex_elim vx22 s1x2 nxtx22.
 ex_elim h_sll_nxtx22s1x2_553x2.
-move=>[phi_sll_x2s_554].
+move=>[phi_sll_x2s_5540].
 move=>[sigma_sll_x2s_554].
 subst.
 move=>H_sll_nxtx22s1x2_553x2.
@@ -109,21 +115,21 @@ ssl_call_pre (f :-> nxtx22 \+ h_sll_nxtx22s1x2_553x2).
 ssl_call (nxtx22, s1x2).
 exists (h_sll_nxtx22s1x2_553x2);
 sslauto.
-move=>h_call13.
+move=>h_call1.
 ex_elim i12.
 ex_elim h_dll_i12s1x2_5551.
-move=>[sigma_call13].
+move=>[sigma_call1].
 subst.
 move=>H_dll_i12s1x2_5551.
 store_valid.
 ssl_read f.
 ssl_open.
 ssl_open_post H_dll_i12s1x2_5551.
-move=>[phi_dll_i12s1x2_5551].
+move=>[phi_dll_i12s1x2_55510].
 move=>[sigma_dll_i12s1x2_5551].
 subst.
 ssl_alloc i2.
-ssl_dealloc (x2).
+ssl_dealloc x2.
 ssl_dealloc (x2 .+ 1).
 ssl_write f.
 ssl_write_post f.
@@ -131,6 +137,8 @@ ssl_write (i2 .+ 1).
 ssl_write_post (i2 .+ 1).
 ssl_write (i2 .+ 2).
 ssl_write_post (i2 .+ 2).
+Hypothesis pure41 : forall vx22, @perm_eq nat_eqType ([:: vx22]) ([:: vx22]).
+Hint Resolve pure41: ssl_pure.
 ssl_write i2.
 ssl_write_post i2.
 ssl_emp;
@@ -146,12 +154,12 @@ sslauto.
 ssl_open_post H_dll_i12s1x2_5551.
 ex_elim vi122 s1i12 wi122.
 ex_elim h_dll_wi122i12s1i12_552i12.
-move=>[phi_dll_i12s1x2_5551].
+move=>[phi_dll_i12s1x2_55510].
 move=>[sigma_dll_i12s1x2_5551].
 subst.
 move=>H_dll_wi122i12s1i12_552i12.
 ssl_alloc i2.
-ssl_dealloc (x2).
+ssl_dealloc x2.
 ssl_dealloc (x2 .+ 1).
 ssl_write (i12 .+ 2).
 ssl_write_post (i12 .+ 2).
@@ -161,6 +169,8 @@ ssl_write (i2 .+ 1).
 ssl_write_post (i2 .+ 1).
 ssl_write (i2 .+ 2).
 ssl_write_post (i2 .+ 2).
+Hypothesis pure42 : forall vx22 vi122 s1i12, @perm_eq nat_eqType ([:: vx22] ++ [:: vi122] ++ s1i12) ([:: vx22] ++ [:: vi122] ++ s1i12).
+Hint Resolve pure42: ssl_pure.
 ssl_write i2.
 ssl_write_post i2.
 ssl_emp;
@@ -175,5 +185,4 @@ unfold_constructor 2;
 exists (vi122), (s1i12), (wi122);
 exists (h_dll_wi122i12s1i12_552i12);
 sslauto.
-
 Qed.
