examples/tree_size.v
@@ -9,11 +9,11 @@ Require Import core.
 
 Inductive tree (x : ptr) (s : seq nat) (h : heap) : Prop :=
 | tree1 of x == null of
-  perm_eq (s) (nil) /\ h = empty
+  @perm_eq nat_eqType (s) (nil) /\ h = empty
 | tree2 of ~~ (x == null) of
   exists (v : nat) (s1 : seq nat) (s2 : seq nat) (l : ptr) (r : ptr),
   exists h_tree_ls1_519 h_tree_rs2_520,
-  perm_eq (s) ([:: v] ++ s1 ++ s2) /\ h = x :-> v \+ x .+ 1 :-> l \+ x .+ 2 :-> r \+ h_tree_ls1_519 \+ h_tree_rs2_520 /\ tree l s1 h_tree_ls1_519 /\ tree r s2 h_tree_rs2_520.
+  @perm_eq nat_eqType (s) ([:: v] ++ s1 ++ s2) /\ h = x :-> v \+ x .+ 1 :-> l \+ x .+ 2 :-> r \+ h_tree_ls1_519 \+ h_tree_rs2_520 /\ tree l s1 h_tree_ls1_519 /\ tree r s2 h_tree_rs2_520.
 
 Inductive treeN (x : ptr) (n : nat) (h : heap) : Prop :=
 | treeN1 of x == null of
@@ -58,19 +58,23 @@ Program Definition tree_size : tree_size_type :=
     )).
 Obligation Tactic := intro; move=>[x r]; ssl_program_simpl.
 Next Obligation.
+Hypothesis tree_perm_eq_trans9: forall x h s_1 s_2, perm_eq s_1 s_2 -> tree x s_1 h -> tree x s_2 h.
+Hint Resolve tree_perm_eq_trans9: ssl_pred.
 ssl_ghostelim_pre.
 move=>n.
 ex_elim h_treeN_xn_a.
-move=>[phi_self].
+move=>[phi_self0].
 move=>[sigma_self].
 subst.
 move=>H_treeN_xn_a.
 ssl_ghostelim_post.
 ssl_open.
 ssl_open_post H_treeN_xn_a.
-move=>[phi_treeN_xn_a].
+move=>[phi_treeN_xn_a0].
 move=>[sigma_treeN_xn_a].
 subst.
+Hypothesis pure10 : 0 == 0.
+Hint Resolve pure10: ssl_pure.
 ssl_emp;
 exists (empty);
 sslauto.
@@ -79,7 +83,7 @@ sslauto.
 ssl_open_post H_treeN_xn_a.
 ex_elim n1x2 n2x2 lx2 rx2 vx2.
 ex_elim h_treeN_lx2n1x2_521x h_treeN_rx2n2x2_522x.
-move=>[phi_treeN_xn_a0][phi_treeN_xn_a1][phi_treeN_xn_a2].
+move=>[phi_treeN_xn_a0] [phi_treeN_xn_a1] [phi_treeN_xn_a2].
 move=>[sigma_treeN_xn_a].
 subst.
 move=>[H_treeN_lx2n1x2_521x H_treeN_rx2n2x2_522x].
@@ -89,9 +93,9 @@ ssl_call_pre (r :-> 0 \+ h_treeN_lx2n1x2_521x).
 ssl_call (n1x2).
 exists (h_treeN_lx2n1x2_521x);
 sslauto.
-move=>h_call3.
+move=>h_call1.
 ex_elim h_treeN_lx2n1x2_521x.
-move=>[sigma_call3].
+move=>[sigma_call1].
 subst.
 move=>H_treeN_lx2n1x2_521x.
 store_valid.
@@ -101,13 +105,15 @@ ssl_call_pre (r :-> 0 \+ h_treeN_rx2n2x2_522x).
 ssl_call (n2x2).
 exists (h_treeN_rx2n2x2_522x);
 sslauto.
-move=>h_call4.
+move=>h_call2.
 ex_elim h_treeN_rx2n2x2_522x.
-move=>[sigma_call4].
+move=>[sigma_call2].
 subst.
 move=>H_treeN_rx2n2x2_522x.
 store_valid.
 ssl_read r.
+Hypothesis pure11 : forall n1x2 n2x2, 0 <= n2x2 -> 0 <= n1x2 -> 0 <= 1 + n1x2 + n2x2 -> 1 + n1x2 + n2x2 == 1 + n1x2 + n2x2.
+Hint Resolve pure11: ssl_pure.
 ssl_write r.
 ssl_write_post r.
 ssl_emp;
@@ -118,5 +124,4 @@ exists (n1x2), (n2x2), (lx2), (rx2), (vx2);
 exists (h_treeN_lx2n1x2_521x);
 exists (h_treeN_rx2n2x2_522x);
 sslauto.
-
 Qed.
