examples/bst_left_rotate.v
@@ -15,47 +15,18 @@ Inductive bst (x : ptr) (sz : nat) (lo : nat) (hi : nat) (h : heap) : Prop :=
   exists h_bst_lsz1lo1hi1_513 h_bst_rsz2lo2hi2_514,
   0 <= sz1 /\ 0 <= sz2 /\ 0 <= v /\ hi == (if hi2 <= v then v else hi2) /\ hi1 <= v /\ lo == (if v <= lo1 then v else lo1) /\ sz == 1 + sz1 + sz2 /\ v <= 7 /\ v <= lo2 /\ h = x :-> v \+ x .+ 1 :-> l \+ x .+ 2 :-> r \+ h_bst_lsz1lo1hi1_513 \+ h_bst_rsz2lo2hi2_514 /\ bst l sz1 lo1 hi1 h_bst_lsz1lo1hi1_513 /\ bst r sz2 lo2 hi2 h_bst_rsz2lo2hi2_514.
 
-
-Hypothesis pure1:
-  forall v2 vr22 hi1 hi1r2 lo1r2 lo2r2,
-    0 <= v2 ->
-    0 <= vr22 ->
-    hi1 <= v2 ->
-    hi1r2 <= vr22 ->
-    v2 <= (if vr22 <= lo1r2 then vr22 else lo1r2) ->
-    v2 <= 7 ->
-    vr22 <= 7 ->
-    vr22 <= lo2r2 ->
-    (if hi1r2 <= v2 then v2 else hi1r2) <= vr22.
-
-Hypothesis pure2:
-  forall v2 vr22 hi1 hi1r2 lo1r2 lo2r2,
-    0 <= v2 ->
-    0 <= vr22 ->
-    hi1 <= v2 ->
-    hi1r2 <= vr22 ->
-    v2 <= (if vr22 <= lo1r2 then vr22 else lo1r2) ->
-    v2 <= 7 ->
-    vr22 <= 7 ->
-    vr22 <= lo2r2 ->
-    v2 <= lo1r2.
-
-Hint Resolve pure1 : ssl_pure.
-Hint Resolve pure2 : ssl_pure.
-
 Definition bst_left_rotate_type :=
   forall (vprogs : ptr * ptr),
-  {(vghosts : nat * nat * nat * ptr * nat * nat * ptr * nat * ptr * nat)},
+  {(vghosts : nat * nat * nat * nat * ptr * nat * ptr * nat * nat * ptr)},
   STsep (
     fun h =>
       let: (x, retv) := vprogs in
-      let: (v, sz2, hi2, unused, hi1, lo2, r, sz1, l, lo1) := vghosts in
+      let: (sz1, sz2, v, hi1, r, lo2, l, lo1, hi2, unused) := vghosts in
       exists h_bst_lsz1lo1hi1_a h_bst_rsz2lo2hi2_b,
-      (* TODO: detect and elide cardinality vars a and b  *)
-      (*0 <= a /\ 0 <= b /\ *)0 <= sz1 /\ 0 <= sz2 /\ 0 <= v /\ hi1 <= v /\ ~~ (r == null) /\ v <= 7 /\ v <= lo2 /\ h = retv :-> unused \+ x :-> v \+ x .+ 1 :-> l \+ x .+ 2 :-> r \+ h_bst_lsz1lo1hi1_a \+ h_bst_rsz2lo2hi2_b /\ bst l sz1 lo1 hi1 h_bst_lsz1lo1hi1_a /\ bst r sz2 lo2 hi2 h_bst_rsz2lo2hi2_b,
+      0 <= sz1 /\ 0 <= sz2 /\ 0 <= v /\ hi1 <= v /\ ~~ (r == null) /\ v <= 7 /\ v <= lo2 /\ h = retv :-> unused \+ x :-> v \+ x .+ 1 :-> l \+ x .+ 2 :-> r \+ h_bst_lsz1lo1hi1_a \+ h_bst_rsz2lo2hi2_b /\ bst l sz1 lo1 hi1 h_bst_lsz1lo1hi1_a /\ bst r sz2 lo2 hi2 h_bst_rsz2lo2hi2_b,
     [vfun (_: unit) h =>
       let: (x, retv) := vprogs in
-      let: (v, sz2, hi2, unused, hi1, lo2, r, sz1, l, lo1) := vghosts in
+      let: (sz1, sz2, v, hi1, r, lo2, l, lo1, hi2, unused) := vghosts in
       exists sz3 sz4 v3 hi3 lo4 lo3 r3 hi4 y,
       exists h_bst_xsz3lo3hi3_515 h_bst_r3sz4lo4hi4_516,
       0 <= sz3 /\ 0 <= sz4 /\ 0 <= v3 /\ hi3 <= v3 /\ sz3 + sz4 == sz1 + sz2 /\ v3 <= 7 /\ v3 <= lo4 /\ h = retv :-> y \+ y :-> v3 \+ y .+ 1 :-> x \+ y .+ 2 :-> r3 \+ h_bst_xsz3lo3hi3_515 \+ h_bst_r3sz4lo4hi4_516 /\ bst x sz3 lo3 hi3 h_bst_xsz3lo3hi3_515 /\ bst r3 sz4 lo4 hi4 h_bst_r3sz4lo4hi4_516
@@ -78,42 +49,45 @@ Program Definition bst_left_rotate : bst_left_rotate_type :=
 Obligation Tactic := intro; move=>[x retv]; ssl_program_simpl.
 Next Obligation.
 ssl_ghostelim_pre.
-move=>[[[[[[[[[v2 sz2] hi2] unused2] hi1] lo2] r2] sz1] l2] lo1].
+move=>[[[[[[[[[sz1 sz2] v2] hi1] r2] lo2] l2] lo1] hi2] unused2].
 ex_elim h_bst_l2sz1lo1hi1_a h_bst_r2sz2lo2hi2_b.
-move=>[phi_self0][phi_self1][phi_self2][phi_self3][phi_self4][phi_self5][phi_self6](*[phi_self7][phi_self8]*).
+move=>[phi_self0] [phi_self1] [phi_self2] [phi_self3] [phi_self4] [phi_self5] [phi_self6].
 move=>[sigma_self].
 subst.
 move=>[H_bst_l2sz1lo1hi1_a H_bst_r2sz2lo2hi2_b].
 ssl_ghostelim_post.
 ssl_read (x .+ 2).
 ssl_open.
-(* TODO: why is the wrong hypothesis used *)
-ssl_open_post H_bst_r2sz2lo2hi2_b. (* H_bst_l2sz1lo1hi1_a *)
 ssl_open_post H_bst_r2sz2lo2hi2_b.
-(*move=>[phi_bst_l2sz1lo1hi1_a].
-move=>[sigma_bst_l2sz1lo1hi1_a].
-subst.
-ssl_open_post H_bst_l2sz1lo1hi1_a.*)
+ssl_open_post H_bst_r2sz2lo2hi2_b.
 ex_elim sz1r2 sz2r2 vr22 hi2r2 hi1r2.
 ex_elim lo1r2 lo2r2 lr22 rr22.
 ex_elim h_bst_lr22sz1r2lo1r2hi1r2_513r2 h_bst_rr22sz2r2lo2r2hi2r2_514r2.
-move=>[phi_bst_l2sz1lo1hi1_a0][phi_bst_l2sz1lo1hi1_a1][phi_bst_l2sz1lo1hi1_a2][phi_bst_l2sz1lo1hi1_a3][phi_bst_l2sz1lo1hi1_a4][phi_bst_l2sz1lo1hi1_a5][phi_bst_l2sz1lo1hi1_a6][phi_bst_l2sz1lo1hi1_a7][phi_bst_l2sz1lo1hi1_a8].
-move=>[sigma_bst_l2sz1lo1hi1_a].
+move=>[phi_bst_r2sz2lo2hi2_b0] [phi_bst_r2sz2lo2hi2_b1] [phi_bst_r2sz2lo2hi2_b2] [phi_bst_r2sz2lo2hi2_b3] [phi_bst_r2sz2lo2hi2_b4] [phi_bst_r2sz2lo2hi2_b5] [phi_bst_r2sz2lo2hi2_b6] [phi_bst_r2sz2lo2hi2_b7] [phi_bst_r2sz2lo2hi2_b8].
+move=>[sigma_bst_r2sz2lo2hi2_b].
 subst.
 move=>[H_bst_lr22sz1r2lo1r2hi1r2_513r2 H_bst_rr22sz2r2lo2r2hi2r2_514r2].
 ssl_read (r2 .+ 1).
+Hypothesis pure1 : forall sz1 sz1r2 sz2r2, 0 <= sz1 -> 0 <= 1 + sz1r2 + sz2r2 -> 0 <= sz2r2 -> 0 <= sz1r2 -> 0 <= 1 + sz1 + sz1r2.
+Hint Resolve pure1: ssl_pure.
+Hypothesis pure2 : forall sz1 sz1r2 sz2r2, 0 <= sz1 -> 0 <= 1 + sz1r2 + sz2r2 -> 0 <= sz2r2 -> 0 <= sz1r2 -> 1 + sz1 + sz1r2 + sz2r2 == sz1 + 1 + sz1r2 + sz2r2.
+Hint Resolve pure2: ssl_pure.
 ssl_write (r2 .+ 1).
 ssl_write_post (r2 .+ 1).
 ssl_write retv.
 ssl_write_post retv.
 ssl_write (x .+ 2).
 ssl_write_post (x .+ 2).
+Hypothesis pure3 : forall lo1r2 vr22 hi1 v2 hi1r2 lo2r2, vr22 <= 7 -> v2 <= (if vr22 <= lo1r2 then vr22 else lo1r2) -> 0 <= v2 -> vr22 <= lo2r2 -> 0 <= vr22 -> hi1r2 <= vr22 -> hi1 <= v2 -> v2 <= 7 -> v2 <= lo1r2.
+Hint Resolve pure3: ssl_pure.
+Hypothesis pure4 : forall lo1r2 vr22 hi1 v2 hi1r2 lo2r2, vr22 <= 7 -> v2 <= (if vr22 <= lo1r2 then vr22 else lo1r2) -> 0 <= v2 -> vr22 <= lo2r2 -> 0 <= vr22 -> hi1r2 <= vr22 -> hi1 <= v2 -> v2 <= 7 -> (if hi1r2 <= v2 then v2 else hi1r2) <= vr22.
+Hint Resolve pure4: ssl_pure.
 ssl_emp;
 exists (1 + sz1 + sz1r2), (sz2r2), (vr22), ((if hi1r2 <= v2 then v2 else hi1r2)), (lo2r2), ((if v2 <= lo1 then v2 else lo1)), (rr22), (hi2r2), (r2);
 exists (x :-> v2 \+ x .+ 1 :-> l2 \+ x .+ 2 :-> lr22 \+ h_bst_l2sz1lo1hi1_a \+ h_bst_lr22sz1r2lo1r2hi1r2_513r2);
 exists (h_bst_rr22sz2r2lo2r2hi2r2_514r2);
 sslauto.
-rewrite (addnC 1) ?addnA; auto. (* why not solvable with //= ? *)
+rewrite (addnC 1) ?addnA; auto. (* TODO: convert to Coq's native nat? *)
 unfold_constructor 2;
 exists (sz1), (sz1r2), (v2), (hi1r2), (hi1), (lo1), (lo1r2), (l2), (lr22);
 exists (h_bst_l2sz1lo1hi1_a);
